Fix Initializers proof in terms of preservation
The missing parts of the proof of Initializers can be solved by stating
some simple block ownership preservation properties on various kinds of
executions, the proofs of which should be simple and similar across
concerned passes.

cfrontend/Csem.v
@@ -858,3 +858,22 @@ Proof.
   eapply external_call_trace_length; eauto.
   inv H; simpl; try omega. eapply external_call_trace_length; eauto.
 Qed.
+
+Definition state_mem (s : state) : option mem :=
+  match s with
+  | State _ _ _ _ m
+  | ExprState _ _ _ _ m
+  | Callstate _ _ _ m
+  | Returnstate _ _ m   => Some m
+  | Stuckstate          => None
+  end.
+
+Lemma star_own_block:
+  forall pol ge s t s',
+  star (step pol) ge s t s' ->
+  forall m m' b cp,
+  state_mem s = Some m ->
+  state_mem s' = Some m' ->
+  Mem.own_block m b cp ->
+  Mem.own_block m' b cp.
+Admitted. (* RB: NOTE: Preservation property. *)
